maj

test2.v
@@ -1,4 +1,5 @@
 Require Import List.
+Require Import PeanoNat.
 
 Locate "<=".
 Print le.
@@ -6,13 +7,17 @@ Print le.
 SearchAbout "eqb".
 SearchAbout "nth".
 Search "fold".
+Search "ltb".
 
 
 Fixpoint insert (x:nat) (l: list nat) : list nat :=
-    match l with
-        | nil => x::nil
-        | h::t => if Nat.ltb x h then x::l else h::(insert x t) 
-    end.
+  match l with
+  | nil => x::nil
+  | h::t => (match Nat.ltb h x with
+            | true => h::(insert x t)
+            | false => x::l
+            end)
+  end.
 
 Fixpoint sort (l: list nat) : list nat :=
     match l with
@@ -20,19 +25,42 @@ Fixpoint sort (l: list nat) : list nat :=
         | h::t => insert h (sort t)
     end.
 
-Definition is_sorted (l:list nat) : Prop := forall x y, x<y -> y < length l -> nth x l 0 <= nth y l 0.
+(* Definition is_sorted (l:list nat) : Prop := forall x y, x<y -> y < length l -> nth x l 0 <= nth y l 0. *)
 
+Print List.hd.
+Print bool.
 
-Definition count (l:list nat) (x:nat) : nat := fold_left (fun c t => if Nat.eqb t (nth x l 0) then c+1 else c) l 0.
+Inductive is_sorted : list nat -> Prop :=
+| nil_sorted : is_sorted nil
+| sing_sorted : forall x, is_sorted (x :: nil)
+| list_sorted : forall h h' t, le h h' -> is_sorted (h'::t) -> is_sorted (h::(h'::t)).
+
+Print fold_left.
+Print nth.
+
+Definition count (l:list nat) (x:nat) : nat := fold_left (fun c h => if Nat.eqb h x then c+1 else c) l 0.
 
 
 Definition are_shuffled (l:list nat) (l':list nat): Prop 
-:= forall x y, x<y -> x < length l -> y < length l' -> count l x = count l' y.
+  := forall x y, x<y -> x < length l -> y < length l' -> count l x = count l' y.
+
+Lemma is_sorted_inv : forall l a, is_sorted (a::l) -> is_sorted l.
+Proof.
+  intros.
+  inversion H.
+  constructor.
+  assumption.
+Qed.
+
+Search "nlt".
+Print Nat.ltb_lt.
+Locate "<?".
+Print lt.
 
 (*
     pose proof eq_nat_decide.
     Search eq_nat.
-   o pose proof eq_nat_is_eq.
+    pose proof eq_nat_is_eq.
 *)
 (* Lemma well_sorted : forall (l : list nat), is_sorted (sort l). *)
 (* Proof. *)
@@ -46,29 +74,125 @@ Definition are_shuffled (l:list nat) (l':list nat): Prop
 (*        (* reflexivity. *) *)
 (* Admitted. *)
 
+Lemma insert_hd : forall l x, is_sorted l -> hd 0 (insert x l) = x \/ hd 0 (insert x l) = hd 0 l.
+Proof.
+  intros.
+  inversion H.
+  simpl; now left.
+  simpl.
+  destruct (x0 <? x).
+  now right.
+  now left.
+  simpl.
+  case (h <? x).
+  now right.
+  now left.
+Qed.
+
 Lemma insert_sort : forall (l: list nat), (is_sorted l) -> forall (x : nat), is_sorted (insert x l).
 Proof.
-  intro l.
+  pose proof Nat.ltb_lt as ltb_lt.
+  pose proof Nat.ltb_nlt as ltb_nlt.
+  pose proof Nat.lt_le_incl as le_implies_lt.
+  pose proof Nat.nlt_ge as nlt_ge.
+  intros.
   induction l.
-  - (* l = nil *)
-    intros.
-    simpl.
-    unfold is_sorted.
-    intros x0 y H0 H1.
-    simpl in H1.
-    unfold lt in H1.
-    inversion H1.
-    subst.
-    inversion H0.
-    inversion H3.
-  -  (* l' = a::l *)
-    intros H x.
-    unfold insert x.
+  simpl; constructor.
+  (* -- is_sorted (insert x l) -- *)
+  assert (is_sorted (insert x l)).
+  apply is_sorted_inv in H.
+  now apply IHl in H.
+  (* ---------------------------- *)
+  (* -------- a <= hd l --------- *)
+  assert (l = nil \/ le a (hd 0 l)).
+  inversion H.
+  now left.
+  now right.
+  (* ---------------------------- *)
+  simpl.
+  case_eq (a <? x).
+  (* --- a < x ----- *)
+  apply is_sorted_inv in H.
+  intro.
+  apply ltb_lt in H2.
+  apply le_implies_lt in H2.
+  apply (insert_hd l x) in H.
+  assert (le a (hd 0 (insert x l))).
+  destruct H as [G1 | G2].
+  now rewrite <- G1 in H2. 
+  destruct l.
+  now simpl.
+  inversion H1.
+  discriminate H.
+  now rewrite G2.
+  apply list_sorted with (t:= tl (insert x l)) in H3.
+  destruct (insert x l).
+  constructor.
+  now simpl in H3.
+  destruct (insert x l).
+  constructor.
+  now simpl in H3.
+  (* ------ ~ (a < x) ------ *)
+  intro.
+  apply ltb_nlt in H2.
+  apply nlt_ge in H2.
+  now constructor.
+Qed.
 
-Lemma count_insert : forall (x: nat) (l : list nat), count (insert x l) = S (count l x).
+Search "eqb".
+(* pose proof eq_nat_decide. *)
+(* pose proof eq_nat_is_eq. *)
 
+Lemma count_lemma : forall l' k x, fold_left (fun c h : nat => if h =? x then c + 1 else c) l' (1+k) = 1 + fold_left (fun c h : nat => if h =? x then c + 1 else c) l' k.
+Proof.
+  induction l'.
+  now simpl.
+  intros.
+  simpl.
+  destruct (a =? x).
+  simpl; rewrite IHl'; simpl.
+  reflexivity.
+  apply IHl'.
+Qed.
+
+Lemma count_insert : forall (x: nat) (l : list nat), count (insert x l) x = S (count l x).
+Proof.
+  pose proof Nat.eqb_eq as eqb_eq.
+  pose proof Nat.eqb_neq as eqb_neq.
+  pose proof Nat.eqb_refl as eqb_refl.
+  pose proof Nat.lt_neq as lt_neq.
+  pose proof Nat.ltb_lt as ltb_lt.
+  assert (forall n m : nat, (n <? m) = true -> n <> m) as ltb_neq.
+  intros.
+  apply lt_neq.
+  now apply ltb_lt.
+  clear lt_neq; clear ltb_lt.
+  unfold count.
+  induction l.
+  simpl.
+  now rewrite eqb_refl.
+  repeat simpl.
+  case_eq (a <? x).
+  intro.
+  apply ltb_neq in H.
+  rewrite <- (eqb_neq a x) in H.
+  simpl; rewrite H; simpl.
+  now apply IHl.
+  intro.
+  case_eq (a =? x).
+  intro.
+  repeat simpl.
+  rewrite eqb_refl; rewrite H0.
+  simpl.
+  apply (count_lemma l 1 x).
+  intro.
+  simpl.
+  rewrite eqb_refl; rewrite H0.
+  simpl.
+  apply (count_lemma l 0 x).
+ Qed.
 
 Lemma sort_shuffled : forall (l : list nat), are_shuffled (sort l).
 Proof.
-
+  
 Qed.
